Added TypeBase theorems to script, which also adds them to TypeBase when loaded.

src/tree/ltreeScript.sml
@@ -14,7 +14,7 @@ structure ltreeScript =
 struct
 
 (*---------------------------------------------------------------------------
- * Declare parent theory structures. 
+ * Declare parent theory structures.
  *---------------------------------------------------------------------------*)
 local open treeTheory combinTheory in end;
 
@@ -99,9 +99,9 @@ local val b = genvar (==`:bool`==)
       val node = (--`node`--)
 in
 fun tree_INDUCT th =
- let val {Bvar,Body} = dest_forall(concl th) 
+ let val {Bvar,Body} = dest_forall(concl th)
      val {ant,conseq} = dest_imp Body
-     val (EVERY, [P, tll]) = strip_comb ant 
+     val (EVERY, [P, tll]) = strip_comb ant
      val concth = SYM(RIGHT_BETA
                    (REFL(mk_comb{Rator=P,Rand=mk_comb{Rator=node,Rand=Bvar}})))
      and IND' = SPEC P tree_Induct
@@ -110,7 +110,7 @@ fun tree_INDUCT th =
      val right = mk_imp{ant=mk_comb{Rator=EVERY_P,  Rand=Bvar}, conseq = b}
      val th1 = SUBST [b |-> concth] (mk_eq{lhs=concl th', rhs=right})
                      (REFL (concl th'))
-      val th2 = GEN Bvar (EQ_MP th1 th') 
+      val th2 = GEN Bvar (EQ_MP th1 th')
    in
    CONV_RULE (ONCE_DEPTH_CONV BETA_CONV) (MP IND' th2)
    end
@@ -133,10 +133,10 @@ val trl = --`trl : tree list`--
 val node = --`node`--
 in
 fun tree_INDUCT_TAC (A,term) =
-   let val {Bvar,Body} = dest_forall term 
+   let val {Bvar,Body} = dest_forall term
        val Afrees = free_varsl A
-       val t' = variant (free_vars term@Afrees) Bvar 
-       val body' = subst [{redex = Bvar, residue = t'}] Body 
+       val t' = variant (free_vars term@Afrees) Bvar
+       val body' = subst [{redex = Bvar, residue = t'}] Body
        val trl = variant (free_vars body'@Afrees) trl
        val asm = --`EVERY (\^t'.^body') trl`--
    in
@@ -161,7 +161,7 @@ val size_thm = prove
  (--`!tl. size ((node tl):tree) = SUC(SUM (MAP size tl))`--,
       REWRITE_TAC [size] THEN
       CONV_TAC SELECT_CONV THEN
-      MP_TAC (SPEC (--`\n. \(tl:(tree)list). SUC(SUM n)`--) 
+      MP_TAC (SPEC (--`\n. \(tl:(tree)list). SUC(SUM n)`--)
                    (INST_TYPE [{redex =  ==`:'b`==, residue = ==`:num`==}]
                               tree_Axiom)) THEN
       REWRITE_TAC [EXISTS_UNIQUE_DEF] THEN
@@ -185,8 +185,8 @@ val Exists_ltree_REP = prove
      REWRITE_TAC [Is_ltree, LENGTH, size_thm, MAP, SUM]);
 
 (* Define the new type.							*)
-val ltree_TY_DEF = 
-  new_type_definition{name = "ltree", 
+val ltree_TY_DEF =
+  new_type_definition{name = "ltree",
                       pred = rator(#Body(dest_exists(concl Exists_ltree_REP))),
                       inhab_thm = Exists_ltree_REP};
 
@@ -211,13 +211,13 @@ val R_11   = prove_rep_fn_one_one ltree_ISO_DEF  and
 
 (* Definition of Node.							*)
 val Node = new_definition("Node",
- --`Node (v:'a) (tl: 'a ltree list) = 
-        (ABS_ltree ((node (MAP (FST o REP_ltree) tl)), 
+ --`Node (v:'a) (tl: 'a ltree list) =
+        (ABS_ltree ((node (MAP (FST o REP_ltree) tl)),
                     ((CONS v (FLAT (MAP (SND o REP_ltree) tl))))))`--);
 
 (* A lemma about Rep_ltree(Node v tl)					*)
-val REP_Node = prove 
- (--`!tl. REP_ltree (Node (v:'a) tl) = 
+val REP_Node = prove
+ (--`!tl. REP_ltree (Node (v:'a) tl) =
          (node (MAP (FST o REP_ltree) tl),
           CONS v (FLAT (MAP (SND o REP_ltree) tl)))`--,
     REWRITE_TAC [Node, SYM(SPEC_ALL R_A), Is_ltree] THEN
@@ -226,7 +226,7 @@ val REP_Node = prove
      POP_ASSUM MP_TAC THEN
      REWRITE_TAC [size_thm, MAP, LENGTH, FLAT, SUM, LENGTH_APPEND] THEN
      REWRITE_TAC [SYM (el 4 (CONJUNCTS ADD_CLAUSES))] THEN
-     DISCH_THEN SUBST1_TAC THEN 
+     DISCH_THEN SUBST1_TAC THEN
      STRIP_TAC THEN STRIP_ASSUME_TAC (SPEC (--`(h:('a)ltree)`--) A_ONTO) THEN
      MP_TAC (SPEC (--`r:^(ty_antiq ty)`--) R_A) THEN
      ASM_REWRITE_TAC [o_THM] THEN
@@ -237,8 +237,8 @@ val REP_Node = prove
      DISCH_THEN SUBST1_TAC THEN REFL_TAC]);
 
 (* A lemma about size and LENGTH of the components of REP_ltree t	*)
-val size_LENGTH_lemma = prove 
- (--`!(t:'a ltree). size (FST (REP_ltree t)) = 
+val size_LENGTH_lemma = prove
+ (--`!(t:'a ltree). size (FST (REP_ltree t)) =
                     LENGTH (SND (REP_ltree t))`--,
     GEN_TAC THEN STRIP_ASSUME_TAC (SPEC (--`t:'a ltree`--) A_ONTO) THEN
     MP_TAC (SPEC_ALL R_A) THEN ASM_REWRITE_TAC [] THEN
@@ -248,9 +248,9 @@ val size_LENGTH_lemma = prove
     REWRITE_TAC [Is_ltree]);
 
 (* Extend the above thm to lists of REP_ltree				*)
-val MAP_size_LENGTH = prove 
- (--`!(tl:'a ltree list). 
-      MAP size (MAP (FST o REP_ltree) tl) = 
+val MAP_size_LENGTH = prove
+ (--`!(tl:'a ltree list).
+      MAP size (MAP (FST o REP_ltree) tl) =
       MAP LENGTH (MAP (SND o REP_ltree) tl)`--,
     LIST_INDUCT_TAC THEN
     ASM_REWRITE_TAC [MAP, size_thm, LENGTH, size_LENGTH_lemma, o_THM]);
@@ -265,7 +265,7 @@ val MAP_size_LENGTH = prove
 (* ---------------------------------------------------------------------*)
 
 val AP = new_recursive_definition
-     {name = "AP", 
+     {name = "AP",
       fixity = Prefix,
       rec_axiom = list_Axiom,
       def = --`(!l. AP NIL l = NIL) /\
@@ -277,7 +277,7 @@ val SPLIT = new_recursive_definition
       fixity = Prefix,
       rec_axiom = num_Axiom,
       def = --`(SPLIT 0 l = (NIL, (l:'a list))) /\
-               (SPLIT (SUC n) l = (CONS (HD l) (FST(SPLIT n (TL l))), 
+               (SPLIT (SUC n) l = (CONS (HD l) (FST(SPLIT n (TL l))),
                                    SND(SPLIT n (TL l))))`--};
 
 val PART = new_recursive_definition
@@ -306,16 +306,16 @@ val NUM_EQ_SYM_EQ = INST_TYPE[{redex= ==`:'a`==,residue= ==`:num`==}] EQ_SYM_EQ
 
 val LENGTH_SND_SPLIT = prove
  (--`!(l:'a list).
-     !n m.(LENGTH l = n+m) ==> 
+     !n m.(LENGTH l = n+m) ==>
           (LENGTH(SND(SPLIT n l)) = m)`--,
-      LIST_INDUCT_TAC THENL 
+      LIST_INDUCT_TAC THENL
       [ONCE_REWRITE_TAC [NUM_EQ_SYM_EQ] THEN
        REWRITE_TAC [LENGTH, ADD_EQ_0] THEN
        REPEAT (STRIP_GOAL_THEN (STRIP_THM_THEN SUBST1_TAC)) THEN
-       REWRITE_TAC [SPLIT, LENGTH], 
+       REWRITE_TAC [SPLIT, LENGTH],
        REWRITE_TAC [LENGTH] THEN STRIP_TAC THEN
        INDUCT_TAC THENL
-       [REWRITE_TAC [ADD_CLAUSES, SPLIT, LENGTH], 
+       [REWRITE_TAC [ADD_CLAUSES, SPLIT, LENGTH],
         REWRITE_TAC [ADD_CLAUSES, INV_SUC_EQ] THEN
 	REPEAT STRIP_TAC THEN RES_TAC THEN
 	ASM_REWRITE_TAC [SPLIT, TL]]]);
@@ -323,50 +323,50 @@ val LENGTH_SND_SPLIT = prove
 
 val LENGTH_FST_SPLIT = prove
  (--`!(l:'a list).
-     !n m.(LENGTH l = n+m) ==> 
+     !n m.(LENGTH l = n+m) ==>
           (LENGTH(FST(SPLIT n l)) = n)`--,
-      LIST_INDUCT_TAC THENL 
+      LIST_INDUCT_TAC THENL
       [ONCE_REWRITE_TAC [NUM_EQ_SYM_EQ] THEN
        REWRITE_TAC [LENGTH, ADD_EQ_0] THEN
        REPEAT (STRIP_GOAL_THEN (STRIP_THM_THEN SUBST1_TAC)) THEN
-       REWRITE_TAC [SPLIT, LENGTH], 
+       REWRITE_TAC [SPLIT, LENGTH],
        REWRITE_TAC [LENGTH] THEN STRIP_TAC THEN
        INDUCT_TAC THENL
-       [REWRITE_TAC [ADD_CLAUSES, SPLIT, LENGTH], 
-        REWRITE_TAC [ADD_CLAUSES, INV_SUC_EQ] THEN 
+       [REWRITE_TAC [ADD_CLAUSES, SPLIT, LENGTH],
+        REWRITE_TAC [ADD_CLAUSES, INV_SUC_EQ] THEN
 	REPEAT STRIP_TAC THEN RES_TAC THEN
 	ASM_REWRITE_TAC [SPLIT, HD, TL, LENGTH]]]);
 
 val APPEND_SPLIT = prove
  (--`!(l:'a list).
-     !n m. (LENGTH l = n + m) ==> 
+     !n m. (LENGTH l = n + m) ==>
            (APPEND (FST(SPLIT n l)) (SND (SPLIT n l)) = l)`--,
-     LIST_INDUCT_TAC THENL 
+     LIST_INDUCT_TAC THENL
      [ONCE_REWRITE_TAC [NUM_EQ_SYM_EQ] THEN
       REWRITE_TAC [LENGTH, ADD_EQ_0] THEN
       REPEAT (STRIP_GOAL_THEN (STRIP_THM_THEN SUBST1_TAC)) THEN
-      REWRITE_TAC [SPLIT, APPEND], 
+      REWRITE_TAC [SPLIT, APPEND],
       REWRITE_TAC [LENGTH] THEN STRIP_TAC THEN
       INDUCT_TAC THENL
-      [REWRITE_TAC [ADD_CLAUSES, SPLIT, APPEND], 
-       REWRITE_TAC [ADD_CLAUSES, INV_SUC_EQ] THEN 
+      [REWRITE_TAC [ADD_CLAUSES, SPLIT, APPEND],
+       REWRITE_TAC [ADD_CLAUSES, INV_SUC_EQ] THEN
        REPEAT STRIP_TAC THEN RES_TAC THEN
        ASM_REWRITE_TAC [SPLIT, HD, TL, APPEND]]]);
 
 
 (* Recursive functions on the REPRESENTATION type...(MAJOR THM)		*)
-val REP_REC_lemma = prove 
- (--`!f. ?!fn. !tl. !l:'a list. 
-     fn(node tl,l):'b = 
+val REP_REC_lemma = prove
+ (--`!f. ?!fn. !tl. !l:'a list.
+     fn(node tl,l):'b =
      f (AP (MAP (\t e.fn(t,e)) tl)(PART (MAP size tl)(TL l)))
-       (HD l :'a) 
+       (HD l :'a)
        (MAP ABS_ltree (AP (MAP $, tl) (PART (MAP size tl) (TL l))))`--,
      STRIP_TAC THEN
      MP_TAC (SPEC (--`\rl:('a list->'b)list. \tl:tree list. \l:'a list.
                     f (AP rl (PART (MAP size tl) (TL l)))
 		      (HD l:'a)
-       	              (MAP ABS_ltree 
-     	      		   (AP (MAP $, tl) 
+       	              (MAP ABS_ltree
+     	      		   (AP (MAP $, tl)
 		               (PART (MAP size tl) (TL l)))):'b`--)
       	          (INST_TYPE[{redex = ==`:'b`==, residue = ==`:'a list->'b`==}]
                             tree_Axiom)) THEN
@@ -374,13 +374,13 @@ val REP_REC_lemma = prove
      CONV_TAC (REDEPTH_CONV BETA_CONV) THEN
      STRIP_TAC THEN CONJ_TAC THENL
      [EXISTS_TAC (--`\p. ((fn (FST p:tree) (SND p:'a list)):'b)`--) THEN
-      CONV_TAC (DEPTH_CONV BETA_CONV) THEN 
+      CONV_TAC (DEPTH_CONV BETA_CONV) THEN
       ASM_REWRITE_TAC [ETA_AX] THEN CONV_TAC (DEPTH_CONV BETA_CONV) THEN
       REPEAT GEN_TAC THEN REFL_TAC,
       REPEAT GEN_TAC THEN
-      POP_ASSUM 
-      (MP_TAC o 
-        SPECL [--`\(t:tree). \(e:'a list). (x(t,e):'b)`--, 
+      POP_ASSUM
+      (MP_TAC o
+        SPECL [--`\(t:tree). \(e:'a list). (x(t,e):'b)`--,
                --`\(t:tree) (e:'a list). (y(t,e):'b)`--]) THEN
       CONV_TAC (REDEPTH_CONV (FUN_EQ_CONV ORELSEC BETA_CONV)) THEN
       REPEAT STRIP_TAC THEN RES_TAC THEN
@@ -389,8 +389,8 @@ val REP_REC_lemma = prove
 
 (* A little simplifying lemma						*)
 val lemma1 = prove
- (--`!(tl:'a ltree list). 
-      (MAP ABS_ltree 
+ (--`!(tl:'a ltree list).
+      (MAP ABS_ltree
            (AP (MAP $,(MAP(FST o REP_ltree)tl))
                (PART (MAP size(MAP(FST o REP_ltree)tl))
                           (FLAT(MAP(SND o REP_ltree)tl))))) = tl`--,
@@ -400,10 +400,10 @@ val lemma1 = prove
 
 (* Another								*)
 val lemma2 = prove
- (--`!(tl:'a ltree list). 
+ (--`!(tl:'a ltree list).
       (AP (MAP(\t e. fn'(t,e))(MAP(FST o REP_ltree)tl))
           (PART (MAP size(MAP(FST o REP_ltree)tl))
-                     (FLAT(MAP(SND o REP_ltree)tl)))) = 
+                     (FLAT(MAP(SND o REP_ltree)tl)))) =
       (MAP (fn' o REP_ltree) tl:('b)list)`--,
     REWRITE_TAC [MAP_size_LENGTH, PART_FLAT] THEN
     LIST_INDUCT_TAC THEN
@@ -413,46 +413,46 @@ val lemma2 = prove
 
 (* Another								*)
 val lemma3 = prove
- (--`!(trl:tree list). !(l:'a list). 
+ (--`!(trl:tree list). !(l:'a list).
       (LENGTH l = SUM(MAP size trl)) ==>
-      (FLAT (MAP (SND o REP_ltree) 
+      (FLAT (MAP (SND o REP_ltree)
             (MAP ABS_ltree (AP (MAP $, trl)
                                (PART(MAP size trl)l)))) = l)`--,
     LIST_INDUCT_TAC THENL
     [REWRITE_TAC [SUM, MAP, LENGTH_NIL] THEN
-     REPEAT STRIP_TAC THEN ASM_REWRITE_TAC [PART, AP, MAP, FLAT], 
+     REPEAT STRIP_TAC THEN ASM_REWRITE_TAC [PART, AP, MAP, FLAT],
      REWRITE_TAC [MAP, SUM, PART] THEN
      REPEAT STRIP_TAC THEN IMP_RES_TAC LENGTH_SND_SPLIT THEN RES_TAC THEN
      IMP_RES_TAC LENGTH_FST_SPLIT THEN
      ASM_REWRITE_TAC [AP, MAP, FLAT, HD, TL, o_THM] THEN
      MP_TAC (SPEC (--`(h:tree),(FST(SPLIT(size h)(l:'a list)))`--) R_A) THEN
-     REWRITE_TAC [Is_ltree] THEN 
+     REWRITE_TAC [Is_ltree] THEN
      POP_ASSUM (ASSUME_TAC o SYM) THEN
-     DISCH_THEN 
-       (fn th1 => FIRST_ASSUM (fn th => (SUBST1_TAC (EQ_MP th1 th)) 
+     DISCH_THEN
+       (fn th1 => FIRST_ASSUM (fn th => (SUBST1_TAC (EQ_MP th1 th))
          handle _ => NO_TAC)) THEN
      IMP_RES_TAC APPEND_SPLIT THEN
      REWRITE_TAC [] THEN POP_ASSUM ACCEPT_TAC]);
 
 (* Another								*)
 val lemma4 = prove
- (--`!(trl:tree list). !(l:'a list). 
+ (--`!(trl:tree list). !(l:'a list).
      (LENGTH l = SUM(MAP size trl)) ==>
-     (node (MAP (FST o REP_ltree) 
-           (MAP ABS_ltree (AP (MAP $, trl) 
+     (node (MAP (FST o REP_ltree)
+           (MAP ABS_ltree (AP (MAP $, trl)
                               (PART(MAP size trl)l)))) = node trl)`--,
     LIST_INDUCT_TAC THENL
     [REWRITE_TAC [SUM, MAP, LENGTH_NIL] THEN
-     REPEAT STRIP_TAC THEN ASM_REWRITE_TAC [PART, AP, MAP], 
+     REPEAT STRIP_TAC THEN ASM_REWRITE_TAC [PART, AP, MAP],
      REWRITE_TAC [MAP, SUM, PART] THEN
      REPEAT STRIP_TAC THEN IMP_RES_TAC LENGTH_SND_SPLIT THEN RES_TAC THEN
      IMP_RES_TAC LENGTH_FST_SPLIT THEN
      ASM_REWRITE_TAC [AP, MAP, FLAT, HD, TL, o_THM] THEN
      MP_TAC (SPEC (--`(h:tree),(FST(SPLIT(size h)(l:'a list)))`--) R_A) THEN
-     REWRITE_TAC [Is_ltree] THEN 
+     REWRITE_TAC [Is_ltree] THEN
      POP_ASSUM (ASSUME_TAC o SYM) THEN
-     DISCH_THEN 
-       (fn th1 => FIRST_ASSUM (fn th => (SUBST1_TAC (EQ_MP th1 th)) 
+     DISCH_THEN
+       (fn th1 => FIRST_ASSUM (fn th => (SUBST1_TAC (EQ_MP th1 th))
            handle _ => NO_TAC)) THEN
      POP_ASSUM (K ALL_TAC) THEN
      POP_ASSUM MP_TAC THEN
@@ -463,9 +463,9 @@ val lemma4 = prove
 val lemma5 = prove
  (--`!trl l.
      (size (node trl) = LENGTH l) ==>
-     (ABS_ltree(node trl,l) = 
-       Node ((HD l):'a) 
-            (MAP ABS_ltree 
+     (ABS_ltree(node trl,l) =
+       Node ((HD l):'a)
+            (MAP ABS_ltree
     	         (AP (MAP $, trl)
                      (PART (MAP size trl) (TL l)))))`--,
      ONCE_REWRITE_TAC [NUM_EQ_SYM_EQ] THEN
@@ -490,10 +490,10 @@ val lemma6 = prove
      ASM_REWRITE_TAC [HD, TL] THEN
      POP_ASSUM (K ALL_TAC) THEN
      POP_ASSUM MP_TAC THEN
-     MAP_EVERY SPEC_TAC [(--`(l':'a list)`--,--`(l:'a list)`--), 
+     MAP_EVERY SPEC_TAC [(--`(l':'a list)`--,--`(l:'a list)`--),
                          (--`(trl:tree list)`--,--`(trl:tree list)`--)] THEN
      LIST_INDUCT_TAC THENL
-     [REWRITE_TAC [MAP, AP, PART, EVERY_DEF], 
+     [REWRITE_TAC [MAP, AP, PART, EVERY_DEF],
      REWRITE_TAC [MAP, SUM, PART] THEN
      REPEAT STRIP_TAC THEN IMP_RES_TAC LENGTH_SND_SPLIT THEN RES_TAC THEN
      ASM_REWRITE_TAC [EVERY_DEF, AP, HD, TL] THEN
@@ -503,8 +503,8 @@ val lemma6 = prove
 
 (* Another								*)
 val lemma7 = prove
- (--`!trl. 
-      EVERY (\t.!l. (size t = LENGTH l) ==> 
+ (--`!trl.
+      EVERY (\t.!l. (size t = LENGTH l) ==>
                     (x(ABS_ltree(t,l)) = y(ABS_ltree(t,l))))
             trl ==>
       (!(l:'a list list).
@@ -513,12 +513,12 @@ val lemma7 = prove
         (MAP x(MAP ABS_ltree(AP(MAP $, trl)l)) :'b list =
          MAP y(MAP ABS_ltree(AP(MAP $, trl)l))))`--,
      LIST_INDUCT_TAC THENL
-     [REWRITE_TAC [EVERY_DEF, MAP, AP], 
+     [REWRITE_TAC [EVERY_DEF, MAP, AP],
       REWRITE_TAC [EVERY_DEF, MAP, AP] THEN
       CONV_TAC (DEPTH_CONV BETA_CONV) THEN
       REWRITE_TAC [] THEN
       REPEAT STRIP_TAC THEN RES_TAC THEN
-      ASM_REWRITE_TAC []]); 
+      ASM_REWRITE_TAC []]);
 
 (* Prove the axiom for 'a ltree						*)
 
@@ -529,7 +529,7 @@ val ltree_Axiom = store_thm("ltree_Axiom",
      CONV_TAC (REDEPTH_CONV BETA_CONV) THEN
      STRIP_TAC THEN CONJ_TAC THENL
      [EXISTS_TAC (--`(fn:^(ty_antiq ty) ->'b) o REP_ltree`--) THEN
-      ASM_REWRITE_TAC [REP_Node, o_THM, TL, HD, lemma1, lemma2], 
+      ASM_REWRITE_TAC [REP_Node, o_THM, TL, HD, lemma1, lemma2],
       REPEAT (POP_ASSUM (K ALL_TAC)) THEN
       REPEAT STRIP_TAC THEN CONV_TAC FUN_EQ_CONV THEN GEN_TAC THEN
       STRIP_ASSUME_TAC (SPEC (--`l:'a ltree`--) A_ONTO) THEN
@@ -538,8 +538,8 @@ val ltree_Axiom = store_thm("ltree_Axiom",
       PURE_REWRITE_TAC [Is_ltree] THEN
       SPEC_TAC (--`SND (r:^(ty_antiq ty))`--,--`(l:'a list)`--) THEN
       SPEC_TAC (--`FST (r:^(ty_antiq ty))`--, --`(t:tree)`--) THEN
-      tree_INDUCT_TAC THEN 
-      REPEAT STRIP_TAC THEN 
+      tree_INDUCT_TAC THEN
+      REPEAT STRIP_TAC THEN
       IMP_RES_THEN SUBST1_TAC lemma5 THEN
       ASM_REWRITE_TAC [] THEN
       IMP_RES_TAC lemma6 THEN
@@ -548,23 +548,23 @@ val ltree_Axiom = store_thm("ltree_Axiom",
 
 
 (* get uniqueness part of ltree_Axiom					*)
-val unique_lemma = 
+val unique_lemma =
    GEN_ALL(CONJUNCT2(CONV_RULE EXISTS_UNIQUE_CONV (SPEC_ALL ltree_Axiom)));
 
 (* Move to conversion nets forces different tactic in this proof. kls. *)
 (* Prove induction thm for 'a ltree					*)
 val ltree_Induct = save_thm("ltree_Induct",
-   let val unique = CONV_RULE (DEPTH_CONV BETA_CONV) unique_lemma 
+   let val unique = CONV_RULE (DEPTH_CONV BETA_CONV) unique_lemma
        val spec = SPECL
-                [--`\b v tl.(EVERY (\x. (x:bool)) b \/ P (Node (v:'a) tl))`--, 
+                [--`\b v tl.(EVERY (\x. (x:bool)) b \/ P (Node (v:'a) tl))`--,
                  --`\(t:'a ltree).T`--,
                  --`(P:'a ltree -> bool)`--]
                 (INST_TYPE [{redex = ==`:'b`==,residue= ==`:bool`==}]
                            (GEN_ALL unique))
-       val conv = CONV_RULE(REDEPTH_CONV(BETA_CONV ORELSEC FUN_EQ_CONV))spec 
+       val conv = CONV_RULE(REDEPTH_CONV(BETA_CONV ORELSEC FUN_EQ_CONV))spec
        val rew1 = prove(--`(X = Y \/ X) = (Y ==> X)`--,
 		        ASM_CASES_TAC (--`X:bool`--) THEN ASM_REWRITE_TAC[])
-       val rew2 = prove(--`(!(h:'a). !t. EVERY P t ==> P(Node h t)) = 
+       val rew2 = prove(--`(!(h:'a). !t. EVERY P t ==> P(Node h t)) =
 			   (!t. EVERY P t ==> !h. P(Node h t))`--,
 		       REPEAT (STRIP_TAC ORELSE EQ_TAC) THEN
 		       RES_TAC THEN FIRST_ASSUM MATCH_ACCEPT_TAC)
@@ -586,20 +586,20 @@ val exists_lemma =
    GEN_ALL(CONJUNCT1(CONV_RULE EXISTS_UNIQUE_CONV (SPEC_ALL ltree_Axiom)));
 
 val Node_11 = store_thm("Node_11",
- --`!(v1:'a). !v2 trl1 trl2. 
+ --`!(v1:'a). !v2 trl1 trl2.
            ((Node v1 trl1) = (Node v2 trl2)) = ((v1 = v2) /\ (trl1 = trl2))`--,
     MP_TAC (SPEC (--`\(l:'a list). \(v:'a). \(trl:'a ltree list). v`--)
 	   (INST_TYPE [{redex = ==`:'b`==, residue = ==`:'a`==}]
                       exists_lemma)) THEN
     MP_TAC (SPEC (--`\l:'a ltree list list.\v:'a.\trl:'a ltree list.trl`--)
-	   (INST_TYPE [{redex = ==`:'b`==, residue = ==`:'a ltree list`==}] 
+	   (INST_TYPE [{redex = ==`:'b`==, residue = ==`:'a ltree list`==}]
                       (GEN_ALL exists_lemma))) THEN
     CONV_TAC (REDEPTH_CONV BETA_CONV) THEN
     REPEAT (STRIP_TAC ORELSE EQ_TAC) THENL
-    [POP_ASSUM (MP_TAC o (AP_TERM (--`(fn':'a ltree->'a)`--))) THEN 
-     ASM_REWRITE_TAC[], 
+    [POP_ASSUM (MP_TAC o (AP_TERM (--`(fn':'a ltree->'a)`--))) THEN
+     ASM_REWRITE_TAC[],
      POP_ASSUM (MP_TAC o (AP_TERM (--`(fn:'a ltree ->'a ltree list)`--))) THEN
-     ASM_REWRITE_TAC[], 
+     ASM_REWRITE_TAC[],
      ASM_REWRITE_TAC[]]);
 
 (* ---------------------------------------------------------------------*)
@@ -617,20 +617,20 @@ val b = genvar(==`:bool`==)
 val alpha = ==`:'a`==
 in
 fun ltree_INDUCT th =
-   let val {Bvar,Body} = dest_forall(concl th) 
+   let val {Bvar,Body} = dest_forall(concl th)
        val {ant,conseq} = dest_imp Body
        val {Bvar = v, Body = con} = dest_forall conseq
-       val (EVERY, [P, tll]) = strip_comb ant 
+       val (EVERY, [P, tll]) = strip_comb ant
        val concth = SYM(RIGHT_BETA(REFL (--`^P(Node ^v ^Bvar)`--)))
        val IND' = SPEC P (INST_TYPE [{redex = alpha, residue = type_of v}]
                                     ltree_Induct)
-       val th' = DISCH ant (SPEC v (UNDISCH(SPEC Bvar th))) 
+       val th' = DISCH ant (SPEC v (UNDISCH(SPEC Bvar th)))
        val th1 = SUBST [b |->  concth]
                        (--`^(concl th') = (EVERY ^P ^Bvar ==> ^b)`--)
-                       (REFL (concl th')) 
-      val th2 = GEN Bvar (DISCH ant (GEN v (UNDISCH (EQ_MP th1 th')))) 
+                       (REFL (concl th'))
+      val th2 = GEN Bvar (DISCH ant (GEN v (UNDISCH (EQ_MP th1 th'))))
   in
-  CONV_RULE (ONCE_DEPTH_CONV BETA_CONV) (MP IND' th2) 
+  CONV_RULE (ONCE_DEPTH_CONV BETA_CONV) (MP IND' th2)
   end
   handle _ => raise ltree_INDUCT_ERR
 end;
@@ -649,16 +649,16 @@ end;
 exception ltree_INDUCT_TAC_ERR;
 
 fun ltree_INDUCT_TAC (A,tm) =
-   let val {Bvar,Body} = dest_forall tm 
+   let val {Bvar,Body} = dest_forall tm
        val Afrees = free_varsl A
-       val t' = variant (free_vars tm@Afrees) Bvar 
+       val t' = variant (free_vars tm@Afrees) Bvar
        val {Args = (t_ty::_),...} = dest_type(type_of Bvar)
-       val body' = subst [{redex = Bvar, residue = t'}] Body 
+       val body' = subst [{redex = Bvar, residue = t'}] Body
        val fv = free_vars body'@Afrees
        val v = mk_var{Name = "v", Ty = t_ty}
        val v' = variant fv v
        val vtrl = mk_var{Name = "trl",
-                         Ty=mk_type{Tyop = "list", 
+                         Ty=mk_type{Tyop = "list",
                                     Args=[mk_type{Tyop="ltree",Args=[t_ty]}]}}
        val trl = variant fv vtrl
        val asm = --`EVERY (\^t'.^body') trl`--
@@ -674,10 +674,55 @@ fun ltree_INDUCT_TAC (A,tm) =
 (* Need this theorem						*)
 val Node_onto = store_thm("Node_onto",
  --`!(t:'a ltree). ?(v:'a). ?trl. t = Node v trl`--,
-     ltree_INDUCT_TAC THEN 
-     STRIP_TAC THEN 
-     MAP_EVERY EXISTS_TAC [--`v:'a`--, --`trl:'a ltree list`--] THEN 
+     ltree_INDUCT_TAC THEN
+     STRIP_TAC THEN
+     MAP_EVERY EXISTS_TAC [--`v:'a`--, --`trl:'a ltree list`--] THEN
      REFL_TAC);
+
+val th0 =
+  GEN_ALL
+   (BETA_RULE
+     (SPEC (Term`\(rl:'b list) (v:'a) (tl:'a ltree list). g v tl:'b`)
+           ltree_Axiom));
+
+val ltree_case_def =
+  Lib.try new_recursive_definition
+    {name = "ltree_case_def",
+     fixity = Prefix,
+     rec_axiom = th0,
+     def = Term `ltree_case f (Node v l) = f v l`};
+
+val ltree_case_cong = store_thm("ltree_case_cong",
+Term `!f g M N.
+         (M = N) /\
+         (!v tl. (N = Node v tl) ==> (f v tl = g v tl))
+           ==>
+         (ltree_case f M = ltree_case g N)`,
+REPEAT GEN_TAC
+  THEN STRUCT_CASES_TAC (SPEC (Term`N:'a ltree`) Node_onto)
+  THEN REPEAT STRIP_TAC
+  THEN ASM_REWRITE_TAC [ltree_case_def]
+  THEN FIRST_ASSUM MATCH_MP_TAC THEN REFL_TAC);
+
+
+val _ = adjoin_to_theory
+{sig_ps = NONE,
+ struct_ps = SOME (fn ppstrm =>
+  let val S = PP.add_string ppstrm
+      fun NL() = PP.add_newline ppstrm
+  in
+    S "val _ = TypeBase.write";             NL();
+    S "  (TypeBase.mk_tyinfo";              NL();
+    S "     {ax=ltree_Axiom,";              NL();
+    S "      case_def=ltree_case_def,";     NL();
+    S "      case_cong=ltree_case_cong,";   NL();
+    S "      induction=ltree_Induct,";      NL();
+    S "      nchotomy=Node_onto,";          NL();
+    S "      size=NONE,";                   NL();
+    S "      one_one=SOME Node_11,";        NL();
+    S "      distinct=NONE});"
+  end)};
+
 
 val _ = export_theory();
 
